feat(KSA): System Key (#1021) (#1055)
Co-authored-by: José Corella <39066999+josecorella@users.noreply.github.com>

AwsCryptographicMaterialProviders/runtimes/java/src/main/smithy-generated/software/amazon/cryptography/keystoreadmin/ToNative.java
@@ -231,6 +231,11 @@ public class ToNative {
     if (dafnyValue.is_CollectionOfErrors()) {
       return ToNative.Error((Error_CollectionOfErrors) dafnyValue);
     }
+    if (dafnyValue.is_AwsCryptographyPrimitives()) {
+      return software.amazon.cryptography.primitives.ToNative.Error(
+        dafnyValue.dtor_AwsCryptographyPrimitives()
+      );
+    }
     if (dafnyValue.is_ComAmazonawsDynamodb()) {
       return software.amazon.cryptography.services.dynamodb.internaldafny.ToNative.Error(
         dafnyValue.dtor_ComAmazonawsDynamodb()
