AwsCryptographicMaterialProviders/dafny/AwsCryptographyKeyStoreAdmin/src/KmsUtils.dfy
@@ -3,11 +3,22 @@
 include "../Model/AwsCryptographyKeyStoreAdminTypes.dfy"
 
 module {:options "/functionSyntax:4" } KmsUtils {
-  import KMS = ComAmazonawsKmsTypes
+  import opened Wrappers
+  import KMS = Com.Amazonaws.Kms
+  import KMSKeystoreOperations
 
   datatype KMSTuple = | KMSTuple(
-    kmsClient: KMS.IKMSClient,
-    grantTokens: KMS.GrantTokenList)
+    kmsClient: KMS.Types.IKMSClient,
+    grantTokens: KMS.Types.GrantTokenList)
+  {
+    ghost predicate ValidState()
+    {
+      && kmsClient.ValidState()
+      && kmsClient.Modifies == kmsClient.Modifies
+      && KMS.Types.IsValid_GrantTokenList(grantTokens)
+    }
+    ghost const Modifies := kmsClient.Modifies
+  }
 
   datatype keyManagerStrat =
     | reEncrypt(reEncrypt: KMSTuple)
@@ -19,6 +30,8 @@ module {:options "/functionSyntax:4" } KmsUtils {
       case reEncrypt(km) =>
         && km.kmsClient.ValidState()
         && km.kmsClient.Modifies == km.kmsClient.Modifies
+        && km.ValidState()
+        && km.Modifies == km.Modifies
       case decryptEncrypt(kmD, kmE) =>
         && kmD.kmsClient.ValidState()
         && kmE.kmsClient.ValidState()
@@ -26,6 +39,72 @@ module {:options "/functionSyntax:4" } KmsUtils {
         && kmE.kmsClient.Modifies == kmE.kmsClient.Modifies
            // We will assume this is the case in order to make verification happy
         && kmE.kmsClient.Modifies !! kmD.kmsClient.Modifies
+        && kmD.ValidState()
+        && kmE.ValidState()
+        && kmD.Modifies == kmD.Modifies
+        && kmE.Modifies == kmE.Modifies
+        && kmD.Modifies !! kmE.Modifies
+    }
+    ghost const Modifies := match this
+      case reEncrypt(km) => km.Modifies
+      case decryptEncrypt(kmD, kmE) =>
+        kmD.Modifies + kmE.Modifies
+  }
+
+  datatype InternalSystemKey =
+    | TrustStorage()
+    | KmsSymEnc(
+        nameonly Tuple: KMSTuple,
+        nameonly KeyId: KMS.Types.KeyIdType
+      )
+  {
+    ghost predicate ValidState()
+    {
+      match this
+      case TrustStorage() => true
+      case KmsSymEnc(Tuple, KeyId) =>
+        && Tuple.ValidState()
+        && KMS.Types.IsValid_KeyIdType(KeyId)
+        && Tuple.Modifies == Tuple.Modifies
+    }
+    ghost const Modifies := match this
+      case TrustStorage() => {}
+      case KmsSymEnc(Tuple, KeyId) => Tuple.Modifies
+  }
+
+  function ExtractKmsOpaque(
+    error: KMSKeystoreOperations.KmsError
+  ): (opaqueError?: Option<KMS.Types.OpaqueError>)
+    ensures
+      && error.ComAmazonawsKms?
+      && error.ComAmazonawsKms.Opaque?
+      ==> opaqueError?.Some? && opaqueError?.value == error.ComAmazonawsKms
+  {
+    match error {
+      case Opaque(obj) => None
+      case KeyManagementException(s) => None
+      case ComAmazonawsKms(comAmazonawsKms: KMS.Types.Error) =>
+        match comAmazonawsKms {
+          case Opaque(obj) => Some(comAmazonawsKms)
+          case OpaqueWithText(obj, objMessage) => Some(comAmazonawsKms)
+          case _ => None
+        }
+    }
+  }
+
+  function ExtractMessageFromKmsError(
+    error: KMSKeystoreOperations.KmsError
+  ): (errorMessage?: Option<string>)
+  {
+    match error {
+      case Opaque(obj) => None
+      case KeyManagementException(s) => Some(s)
+      case ComAmazonawsKms(comAmazonawsKms: KMS.Types.Error) =>
+        match comAmazonawsKms {
+          case Opaque(obj) => None
+          case OpaqueWithText(obj, objMessage) => Some(objMessage)
+          case _ => comAmazonawsKms.message
+        }
     }
   }
 }
