AwsCryptographicMaterialProviders/dafny/AwsCryptographyKeyStore/test/CleanupItems.dfy
@@ -9,6 +9,7 @@ module CleanupItems {
   import opened Wrappers
   import opened Fixtures
   import Structure
+  import UTF8
 
   method DeleteVersion(
     branchKeyIdentifier: string,
@@ -112,5 +113,33 @@ module CleanupItems {
     return Success(true);
   }
 
+  method DeleteBranchKeyWithOneVersion(
+    Identifier: string,
+    ddbClient: DDB.Types.IDynamoDBClient,
+    tableName: string := branchKeyStoreName
+  )
+    returns (output: Result<bool, DDB.Types.Error>)
+    requires
+      && ddbClient.ValidState()
+      && DDB.Types.IsValid_TableName(tableName)
+      && UTF8.IsASCIIString(tableName)
+    modifies ddbClient.Modifies
+    ensures ddbClient.ValidState()
+  {
+    var storage :- expect Fixtures.DefaultStorage(
+      physicalName := tableName,
+      logicalName := tableName,
+      ddbClient?:=Some(ddbClient));
+    var lastActiveInput := Types.GetEncryptedActiveBranchKeyInput(Identifier:=Identifier);
+    var lastActive? :- expect storage.GetEncryptedActiveBranchKey(lastActiveInput);
+    expect lastActive?.Item.Type.ActiveHierarchicalSymmetricVersion?;
+    var lastActive := lastActive?.Item.Type.ActiveHierarchicalSymmetricVersion.Version;
+    var _ := DeleteTypeWithFailure(Identifier, Structure.BRANCH_KEY_ACTIVE_TYPE, ddbClient);
+    var _ := DeleteTypeWithFailure(Identifier, Structure.BEACON_KEY_TYPE_VALUE, ddbClient);
+    var _ := DeleteTypeWithFailure(Identifier, Structure.MUTATION_COMMITMENT_TYPE, ddbClient);
+    var _ := DeleteTypeWithFailure(Identifier, Structure.MUTATION_INDEX_TYPE, ddbClient);
+    var _ := DeleteTypeWithFailure(Identifier, Structure.BRANCH_KEY_TYPE_PREFIX + lastActive, ddbClient);
+    return Success(true);
+  }
 
 }
